Code refactoring regarding readability:
1. Created a predicate UniqueSenders that checks whether
   all messages in a set are from different senders. It is
   now used in all necessary places in messages.dfy
2. committedClientOperations is taken out of the Working Window
   and placed in the variables of the Replica. Also it no longer
   holds Option as the value associated with each key. Now that it
   is a finite map, the things that have not yet been committed
   simply are not present in the map.
3. Clearing the Working Window now happens in one step - EmptyWorkingWindow.
   This function takes care of clearing the votes we no longer need after
   View Change is initiated.

docs/sbft-formal-model/messages.dfy
@@ -43,11 +43,7 @@ module Messages {
       || (&& |votes| == quorumSize
           && WF()
           && (forall v | v in votes :: v.payload == prototype()) // messages have to be votes that match eachother by the prototype 
-          && (forall v1, v2 | && v1 in votes
-                              && v2 in votes
-                              && v1 != v2
-                                :: v1.sender != v2.sender) // unique senders
-          )
+          && UniqueSenders(votes))
     }
     predicate empty() {
       && |votes| == 0
@@ -60,10 +56,7 @@ module Messages {
       && (forall v | v in msgs :: && v.payload.ViewChangeMsg?
                                   && v.payload.validViewChangeMsg(quorumSize)
                                   && v.payload.newView == view) // All the ViewChange messages have to be for the same View. 
-      && (forall v1, v2 | && v1 in msgs
-                          && v2 in msgs
-                          && v1 != v2
-                            :: v1.sender != v2.sender) // unique senders
+      && UniqueSenders(msgs)
       && |msgs| == quorumSize //TODO: once proof is complete try with >=
     }
   }
@@ -73,12 +66,16 @@ module Messages {
       && |msgs| > 0
       && (forall m | m in msgs :: && m.payload.CheckpointMsg?
                                   && m.payload.seqIDReached == lastStableCheckpoint)
-      && (forall m1, m2 | && m1 in msgs
-                          && m2 in msgs
-                          && m1 != m2
-                            :: m1.sender != m2.sender) // unique senders
+      && UniqueSenders(msgs)
       && |msgs| >= quorumSize
     }
+  }
+
+  predicate UniqueSenders(msgs:set<Network.Message<Message>>) {
+    (forall m1, m2 | && m1 in msgs
+                     && m2 in msgs
+                     && m1 != m2
+                       :: m1.sender != m2.sender)
   }
 
   // Define your Message datatype here.
